Công thức:  h(x) = (2 * x + 5) mod 11

a)
h(12) = 7
h(44) = 5
h(13) = 9
h(88) = 5
h(23) = 7
h(94) = 6
h(11) = 5 
h(39) = 5
h(20) = 1
h(16) = 4
h(5) = 4

Vị trí                          Chaining
  0                                
  1                                20
  2                                
  3                                
  4                                16-->5
  5                                44-->88-->11-->39
  6                                94
  7                                12-->23
  8                                
  9                                13
 10                                

b) 

h(12) = 7 
h(44) = 5
h(13) = 9
h(88) = 5 --> 6
h(23) = 7 --> 8
h(94) = 6 --> 10
h(11) = 5 --> 4
h(39) = 5 --> 3
h(20) = 1 
h(16) = 4 --> 2 
h(5)  = 4 --> 0

Vị trí                          linear probing
  0                                   5
  1                                   20
  2                                   16
  3                                   39
  4                                   11
  5                                   44
  6                                   88 
  7                                   12  
  8                                   23  
  9                                   13 
 10                                   94  