Công thức h(X) = (X + 3) mod 17

a)

h(1) = 4
h(3) = 6
h(18) = 4
h(8) = 11
h(23) = 9
h(35) = 4
h(11) = 14
h(36) = 5
h(20) = 6
h(16) = 2

Vị trí                          Chaining
  0                                
  1                                
  2                                16
  3                                
  4                                1-->18-->35
  5                                36
  6                                3-->20
  7                                
  8                                
  9                                23
 10                                
 11                                8
 12                                
 13                                
 14                                11
 15                                
 16                                

 b)

h(1) = 4
h(3) = 6
h(18)= 4 --> 3
h(8) = 11
h(23)= 9
h(35)= 4 --> 5 
h(11)= 14
h(36)= 5 --> 7
h(20)= 6 --> 8
h(16)= 2

Vị trí                       linear probing
  0                                
  1                                
  2                                16
  3                                18
  4                                1
  5                                35
  6                                3
  7                                36
  8                                20
  9                                23
 10                                
 11                                8
 12                                
 13                                
 14                                11                            




